progress on recover_idem
Proved Lemma crash_xform_list2nmem : forall vl (F : rawpred),

  crash_xform F (list2nmem vl) ->
    exists vsl, F (list2nmem vsl) /\ length vl = length vsl.

However, this isn't quite useful as we know too little about vsl
other than that its length is equal to vl.

In recover_idem, Get stuck on goal:

    H1 : [[[ vl ::: Fold ]]]
    H2 : length vsl = length vl
    ----------------------------------------------------
    crash_xform (rep_inner xp x   (Synced vsl) x0) =p=>
    crash_xform (rep_inner xp ?x3 (Synced vl) ?x7) * [[[ vl :: Fold ]]]
                                         ^^^^           ^^^^

A stronger fact like

   exisits vsl, ... /\ possible_crash_list vsl (map fst vl)

might help, but I cannot prove this too.
(see crash_xform_list2nmem_possible_crash_list in GenSepN.v)

src/Pred.v
@@ -1831,4 +1831,25 @@ Proof.
   rewrite H5; auto; discriminate.
 Qed.
 
+
+(* exclude an address from a predicate *)
+Definition pred_ex AT AEQ V (F : @pred AT AEQ V) a : @pred AT AEQ V :=
+  fun m => exists v, F (upd m a v).
+
+Lemma pred_ex_mem_except : forall AT AEQ V (F : @pred AT AEQ V) m a,
+  F m -> indomain a m -> (pred_ex F a) (mem_except m a).
+Proof.
+  unfold pred_ex; intros.
+  case_eq (m a); intros.
+
+  exists v.
+  replace (upd (mem_except m a) a v) with m; auto.
+  apply functional_extensionality; intros.
+  unfold upd, mem_except.
+  destruct (AEQ x a); subst; auto.
+
+  unfold indomain in H0; destruct H0.
+  congruence.
+Qed.
+
 Global Opaque pred.
